---
layout: post
title: MathJax
---

As I embark on the PyESL project, I'll need to include math equations in future blog posts. The easiest way to accomplish this is to use MathJax so that I can incorporate Tex/LaTeX/MathML-based equations within HTML. In Jekyll, all you need to do is add the MathJax javascript to the header section of your default.html and add a new variable to your _config.yml file.
<br><br>
 
    <head>
        ...
        <script type="text/javascript" src="http://cdn.mathjax.org/mathjax/latest/MathJax.js?config=TeX-AMS-MML_HTMLorMML">
    </script>
        ...
    </head>

<br>
and add the following to your _config.yml file:
<br><br>

    markdown: kramdown

<br>
For example, this markdown:
<br><br>

    Inline equation \\( {y} = {m}{x} + {b} \\) and block equation \\[ {y} = {m}{x}+{b} \\] 

<br>
produces:
<br><br>

<i>Inline equation \\( {y} = {m}{x}+{b} \\) and block equation \\[ {y} = {m}{x}+{b} \\] </i>

Here, the parentheses denote an inline equation while the square brackets denote a block equation.

<br>

And this is a multiline equation:
<!--more-->

\\[
\begin{align} 
{RSS} &= (\textbf{Y} - \textbf{X}{\beta})^{T}(\textbf{Y} - \textbf{X}{\beta}) \\\
&= \textbf{Y}^{T}\textbf{Y} - \textbf{Y}^{T}\textbf{X}{\beta} - {\beta}^{T}\textbf{X}^{T}\textbf{Y} + {\beta}^{T}\textbf{X}^{T}\textbf{X}{\beta} \qquad \because\textbf{AB}^{T}=\textbf{B}^{T}\textbf{A}^{T} \\\
&= \textbf{Y}^{T}\textbf{Y} - 2\textbf{Y}^{T}\textbf{X}{\beta} + {\beta}^{T}\textbf{X}^{T}\textbf{X}{\beta} \qquad \because \textbf{Y}^{T}\textbf{X}{\beta} = \textbf{X}^{T}{\beta}^{T}\textbf{Y} \\\
\end{align}
\\]

Taking the derivative and solving for \\( {\beta} \\):

\\[
\begin{align} 
\frac{dRSS}{d\beta} &= - 2\textbf{Y}^{T}\textbf{X} + \textbf{X}^{T}\textbf{X}{\beta} + {\beta}^{T}\textbf{X}^{T}\textbf{X} \\\
0 &=  - 2\textbf{Y}^{T}\textbf{X} + 2{\beta}^{T}\textbf{X}^{T}\textbf{X} \qquad \because \textbf{X}^{T}\textbf{X}{\beta} = {\beta}^{T}\textbf{X}^{T}\textbf{X} \\\
0 &=  - \textbf{Y}^{T}\textbf{X} + {\beta}^{T}\textbf{X}^{T}\textbf{X} \\\
0 &=  - \textbf{X}^{T}\textbf{Y} + \textbf{X}^{T}\textbf{X}{\beta} \qquad \because\textbf{AB}^{T}=\textbf{B}^{T}\textbf{A}^{T} \\\
\textbf{X}^{T}\textbf{X}{\beta} &= \textbf{X}^{T}\textbf{Y} \\\
{\beta} &= (\textbf{X}^{T}\textbf{X})^{-1}\textbf{X}^{T}\textbf{Y}
\end{align}
\\]
